Unifying the variable naming of sequences

src/Collections/Sequences/Seq.dfy
@@ -28,49 +28,49 @@ module Seq {
   ***********************************************************/
 
   /* finds the first element in the sequence */
-  function method First<T>(s: seq<T>): T
-    requires |s| > 0
+  function method First<T>(xs: seq<T>): T
+    requires |xs| > 0
   {
-    s[0]
+    xs[0]
   }
 
-  function method DropFirst<T>(s: seq<T>): seq<T>
-    requires |s| > 0
+  function method DropFirst<T>(xs: seq<T>): seq<T>
+    requires |xs| > 0
   {
-    s[1..]
+    xs[1..]
   }
 
   /* finds the last element in the sequence */
-  function method Last<T>(s: seq<T>): T
-    requires |s| > 0;
+  function method Last<T>(xs: seq<T>): T
+    requires |xs| > 0;
   {
-    s[|s|-1]
+    xs[|xs|-1]
   }
 
   /* returns the sequence slice up to but not including the last element */
-  function method DropLast<T>(s: seq<T>): seq<T> 
-    requires |s| > 0;
+  function method DropLast<T>(xs: seq<T>): seq<T> 
+    requires |xs| > 0;
   {
-    s[..|s|-1]
+    xs[..|xs|-1]
   }
 
   /* concatenating everything but the last element + the last element results in the original seq */
-  lemma LemmaLast<T>(s: seq<T>)
-    requires |s| > 0;
-    ensures  DropLast(s) + [Last(s)] == s;
+  lemma LemmaLast<T>(xs: seq<T>)
+    requires |xs| > 0;
+    ensures  DropLast(xs) + [Last(xs)] == xs;
   {
   }
 
   /* the last element in an appended sequence will be the last element of the latter sequence */
-  lemma LemmaAppendLast<T>(a: seq<T>, b: seq<T>)
-    requires 0 < |a + b| && 0 < |b|
-    ensures Last(a + b) == Last(b)
+  lemma LemmaAppendLast<T>(xs: seq<T>, ys: seq<T>)
+    requires 0 < |xs + ys| && 0 < |ys|
+    ensures Last(xs + ys) == Last(ys)
   {
   }
 
   /* explains associative property of sequences in addition */
-  lemma LemmaConcatIsAssociative<T>(a: seq<T>, b: seq<T>, c: seq<T>)
-    ensures a + (b + c) == (a + b) + c;
+  lemma LemmaConcatIsAssociative<T>(xs: seq<T>, ys: seq<T>, zs: seq<T>)
+    ensures xs + (ys + zs) == (xs + ys) + zs;
   {
   }
 
@@ -80,44 +80,44 @@ module Seq {
   *
   ***********************************************************/
   
-  predicate IsPrefix<T>(a: seq<T>, b: seq<T>)
-    ensures IsPrefix(a, b) ==> (|a| <= |b| && a == b[..|a|])
+  predicate IsPrefix<T>(xs: seq<T>, ys: seq<T>)
+    ensures IsPrefix(xs, ys) ==> (|xs| <= |ys| && xs == ys[..|xs|])
   {
-    a <= b    
+    xs <= ys    
   }
   
-  predicate IsSuffix<T>(a: seq<T>, b: seq<T>)
+  predicate IsSuffix<T>(xs: seq<T>, ys: seq<T>)
   {
-    && |a| <= |b|
-    && a == b[|b|-|a|..]
+    && |xs| <= |ys|
+    && xs == ys[|ys|-|xs|..]
   }
 
   /* a sequence that is sliced at the jth element concatenated with that same
   sequence sliced from the jth element is equal to the original, unsliced sequence */
-  lemma LemmaSplitAt<T>(s: seq<T>, pos: nat)
-    requires pos < |s|;
-    ensures s[..pos] + s[pos..] == s;
+  lemma LemmaSplitAt<T>(xs: seq<T>, pos: nat)
+    requires pos < |xs|;
+    ensures xs[..pos] + xs[pos..] == xs;
   {
   }
 
   /* ensures that the element from a slice is included in the original sequence */
-  lemma LemmaElementFromSlice<T>(s: seq<T>, s':seq<T>, a: int, b: int, pos: nat)
-    requires 0 <= a <= b <= |s|;
-    requires s' == s[a..b];
+  lemma LemmaElementFromSlice<T>(xs: seq<T>, ys:seq<T>, a: int, b: int, pos: nat)
+    requires 0 <= a <= b <= |xs|;
+    requires ys == xs[a..b];
     requires a <= pos < b;
-    ensures  pos - a < |s'|;
-    ensures  s'[pos-a] == s[pos];
+    ensures  pos - a < |ys|;
+    ensures  ys[pos-a] == xs[pos];
   {
   }
 
-  lemma LemmaSliceOfSlice<T>(s: seq<T>, s1: int, e1: int, s2: int, e2: int)
-    requires 0 <= s1 <= e1 <= |s|;
+  lemma LemmaSliceOfSlice<T>(xs: seq<T>, s1: int, e1: int, s2: int, e2: int)
+    requires 0 <= s1 <= e1 <= |xs|;
     requires 0 <= s2 <= e2 <= e1 - s1;
-    ensures  s[s1..e1][s2..e2] == s[s1+s2..s1+e2];
+    ensures  xs[s1..e1][s2..e2] == xs[s1+s2..s1+e2];
   {
-    var r1 := s[s1..e1];
+    var r1 := xs[s1..e1];
     var r2 := r1[s2..e2];
-    var r3 := s[s1+s2..s1+e2];
+    var r3 := xs[s1+s2..s1+e2];
     assert |r2| == |r3|;
     forall i {:trigger r2[i], r3[i]}| 0 <= i < |r2| ensures r2[i] == r3[i];
     {
@@ -125,214 +125,214 @@ module Seq {
   }
 
   /* converts a sequence to an array */
-  method ToArray<T>(s: seq<T>) returns (a: array<T>)
+  method ToArray<T>(xs: seq<T>) returns (a: array<T>)
     ensures fresh(a)
-    ensures a.Length == |s|
-    ensures forall i :: 0 <= i < |s| ==> a[i] == s[i]
+    ensures a.Length == |xs|
+    ensures forall i :: 0 <= i < |xs| ==> a[i] == xs[i]
   {
-    a := new T[|s|](i requires 0 <= i < |s| => s[i]);
+    a := new T[|xs|](i requires 0 <= i < |xs| => xs[i]);
   }
 
   /* converts a sequence to a set */
-  function method {:opaque} ToSet<T>(s: seq<T>): set<T> 
+  function method {:opaque} ToSet<T>(xs: seq<T>): set<T> 
   {
-    set x: T | x in s
+    set x: T | x in xs
   }
 
   /* proves that the cardinality of a subsequence is always less than or equal to that
   of the full sequence */
-  lemma LemmaCardinalityOfSet<T>(s: seq<T>)
-    ensures |ToSet(s)| <= |s| 
+  lemma LemmaCardinalityOfSet<T>(xs: seq<T>)
+    ensures |ToSet(xs)| <= |xs| 
   {
     reveal ToSet();
-    if |s| == 0 {
+    if |xs| == 0 {
     } else {
-      assert ToSet(s) == ToSet(DropLast(s)) + {Last(s)};
-      LemmaCardinalityOfSet(DropLast(s));
+      assert ToSet(xs) == ToSet(DropLast(xs)) + {Last(xs)};
+      LemmaCardinalityOfSet(DropLast(xs));
     }
   }
   
   /* the cardinality of a subsequence of an empty sequence is also 0 */
-  lemma LemmaCardinalityOfEmptySetIs0<T>(s: seq<T>)
-    ensures |ToSet(s)| == 0 <==> |s| == 0
+  lemma LemmaCardinalityOfEmptySetIs0<T>(xs: seq<T>)
+    ensures |ToSet(xs)| == 0 <==> |xs| == 0
   {
     reveal ToSet();
-    if |s| != 0 {
-      assert s[0] in ToSet(s);
+    if |xs| != 0 {
+      assert xs[0] in ToSet(xs);
     }
   }
 
   /* is true if there are no duplicate values in the sequence */
-  predicate {:opaque} HasNoDuplicates<T>(s: seq<T>) 
+  predicate {:opaque} HasNoDuplicates<T>(xs: seq<T>) 
   {
-    (forall i, j {:trigger s[i], s[j]}:: 0 <= i < |s| && 0 <= j < |s| && i != j ==> s[i] != s[j])
+    (forall i, j {:trigger xs[i], xs[j]}:: 0 <= i < |xs| && 0 <= j < |xs| && i != j ==> xs[i] != xs[j])
   }
 
-  /* if sequence a and b don't have duplicates and there are no elements in
-  common between them, then the concatenated sequence of a + b will not contain
+  /* if sequences xs and ys don't have duplicates and there are no elements in
+  common between them, then the concatenated sequence of xs + ys will not contain
   duplicates either */
-  lemma {:timeLimitMultiplier 3} LemmaNoDuplicatesInConcat<T>(a: seq<T>, b: seq<T>)
-    requires HasNoDuplicates(a);
-    requires HasNoDuplicates(b);
-    requires multiset(a) !! multiset(b);
-    ensures HasNoDuplicates(a+b);
+  lemma {:timeLimitMultiplier 3} LemmaNoDuplicatesInConcat<T>(xs: seq<T>, ys: seq<T>)
+    requires HasNoDuplicates(xs);
+    requires HasNoDuplicates(ys);
+    requires multiset(xs) !! multiset(ys);
+    ensures HasNoDuplicates(xs+ys);
   {
     reveal HasNoDuplicates();
-    var c := a + b;
-    if |c| > 1 {
-      assert forall i, j {:trigger c[i], c[j]}:: i != j && 0 <= i < |a| && |a| <= j < |c| ==>
-        c[i] in multiset(a) && c[j] in multiset(b) && c[i] != c[j]; 
+    var zs := xs + ys;
+    if |zs| > 1 {
+      assert forall i, j {:trigger zs[i], zs[j]}:: i != j && 0 <= i < |xs| && |xs| <= j < |zs| ==>
+        zs[i] in multiset(xs) && zs[j] in multiset(ys) && zs[i] != zs[j]; 
     }
   }
 
   /* A sequence with no duplicates converts to a set of the same cardinality */
-  lemma LemmaCardinalityOfSetNoDuplicates<T>(s: seq<T>)
-    requires HasNoDuplicates(s)
-    ensures |ToSet(s)| == |s|
+  lemma LemmaCardinalityOfSetNoDuplicates<T>(xs: seq<T>)
+    requires HasNoDuplicates(xs)
+    ensures |ToSet(xs)| == |xs|
   {
     reveal HasNoDuplicates();
     reveal ToSet();
-    if |s| == 0 {
+    if |xs| == 0 {
     } else {
-      LemmaCardinalityOfSetNoDuplicates(DropLast(s));
-      assert ToSet(s) == ToSet(DropLast(s)) + {Last(s)};
+      LemmaCardinalityOfSetNoDuplicates(DropLast(xs));
+      assert ToSet(xs) == ToSet(DropLast(xs)) + {Last(xs)};
     }
   }
 
   /* A sequence with cardinality equal to its set has no duplicates */
-  lemma LemmaNoDuplicatesCardinalityOfSet<T>(s: seq<T>)
-    requires |ToSet(s)| == |s|
-    ensures HasNoDuplicates(s)
+  lemma LemmaNoDuplicatesCardinalityOfSet<T>(xs: seq<T>)
+    requires |ToSet(xs)| == |xs|
+    ensures HasNoDuplicates(xs)
   {
     reveal HasNoDuplicates();
     reveal ToSet();
-    if |s| == 0 {
+    if |xs| == 0 {
     } else {
-      assert s == [First(s)] + DropFirst(s);
-      assert ToSet(s) == {First(s)} + ToSet(DropFirst(s));
-      if First(s) in DropFirst(s) {
+      assert xs == [First(xs)] + DropFirst(xs);
+      assert ToSet(xs) == {First(xs)} + ToSet(DropFirst(xs));
+      if First(xs) in DropFirst(xs) {
         // If there is a duplicate, then we show that |ToSet(s)| == |s| cannot hold.
-        assert ToSet(s) == ToSet(DropFirst(s));
-        LemmaCardinalityOfSet(DropFirst(s));
-        assert |ToSet(s)| <= |DropFirst(s)|;
+        assert ToSet(xs) == ToSet(DropFirst(xs));
+        LemmaCardinalityOfSet(DropFirst(xs));
+        assert |ToSet(xs)| <= |DropFirst(xs)|;
       } else {
-        assert |ToSet(s)| == 1 + |ToSet(DropFirst(s))|;
-        LemmaNoDuplicatesCardinalityOfSet(DropFirst(s));
+        assert |ToSet(xs)| == 1 + |ToSet(DropFirst(xs))|;
+        LemmaNoDuplicatesCardinalityOfSet(DropFirst(xs));
       }
     }
   }
 
   /* proves that there are no duplicate values in the multiset version of the sequence */
-  lemma LemmaMultisetHasNoDuplicates<T>(s: seq<T>)
-    requires HasNoDuplicates(s)
-    ensures forall x {:trigger multiset(s)[x]} | x in multiset(s):: multiset(s)[x] == 1
+  lemma LemmaMultisetHasNoDuplicates<T>(xs: seq<T>)
+    requires HasNoDuplicates(xs)
+    ensures forall x {:trigger multiset(xs)[x]} | x in multiset(xs):: multiset(xs)[x] == 1
   {
-    if |s| == 0 {
+    if |xs| == 0 {
     } else {
-      assert s == DropLast(s) + [Last(s)];
-      assert Last(s) !in DropLast(s) by {
+      assert xs == DropLast(xs) + [Last(xs)];
+      assert Last(xs) !in DropLast(xs) by {
         reveal HasNoDuplicates();
       }
-      assert HasNoDuplicates(DropLast(s)) by {
+      assert HasNoDuplicates(DropLast(xs)) by {
         reveal HasNoDuplicates();
       }
-      LemmaMultisetHasNoDuplicates(DropLast(s));
+      LemmaMultisetHasNoDuplicates(DropLast(xs));
     }
   }
 
   /* finds the index of the first occurrence of an element in the sequence */
-  function method {:opaque} IndexOf<T(==)>(s: seq<T>, v: T): (i: nat)
-    requires v in s
-    ensures i < |s| && s[i] == v
-    ensures forall j {:trigger s[j]} :: 0 <= j < i ==> s[j] != v
+  function method {:opaque} IndexOf<T(==)>(xs: seq<T>, v: T): (i: nat)
+    requires v in xs
+    ensures i < |xs| && xs[i] == v
+    ensures forall j {:trigger xs[j]} :: 0 <= j < i ==> xs[j] != v
   {
-    if s[0] == v then 0 else 1 + IndexOf(s[1..], v)
+    if xs[0] == v then 0 else 1 + IndexOf(xs[1..], v)
   }
 
   /* finds the index of the first occurrence of an element in the sequence if
   found */
-  function method {:opaque} IndexOfOption<T(==)>(s: seq<T>, v: T): (o: Option<nat>)
-    ensures if o.Some? then o.value < |s| && s[o.value] == v &&
-                            forall j {:trigger s[j]} :: 0 <= j < o.value ==> s[j] != v
-            else v !in s
+  function method {:opaque} IndexOfOption<T(==)>(xs: seq<T>, v: T): (o: Option<nat>)
+    ensures if o.Some? then o.value < |xs| && xs[o.value] == v &&
+                            forall j {:trigger xs[j]} :: 0 <= j < o.value ==> xs[j] != v
+            else v !in xs
   {
-    if |s| == 0 then None()
+    if |xs| == 0 then None()
     else
-      if s[0] == v then Some(0)
+      if xs[0] == v then Some(0)
       else
-        var o' := IndexOfOption(s[1..], v);
+        var o' := IndexOfOption(xs[1..], v);
         if o'.Some? then Some(o'.value + 1) else None()
   }
 
   /* finds the index of the last occurrence of an element in the sequence */
-  function method {:opaque} LastIndexOf<T(==)>(s: seq<T>, v: T): (i: nat)
-    requires v in s
-    ensures i < |s| && s[i] == v
-    ensures forall j {:trigger s[j]} :: i < j < |s| ==> s[j] != v
+  function method {:opaque} LastIndexOf<T(==)>(xs: seq<T>, v: T): (i: nat)
+    requires v in xs
+    ensures i < |xs| && xs[i] == v
+    ensures forall j {:trigger xs[j]} :: i < j < |xs| ==> xs[j] != v
   {
-    if s[|s|-1] == v then |s| - 1 else LastIndexOf(s[..|s|-1], v)
+    if xs[|xs|-1] == v then |xs| - 1 else LastIndexOf(xs[..|xs|-1], v)
   }
 
   /* finds the index of the last occurrence of an element in the sequence if
   found */
-  function method {:opaque} LastIndexOfOption<T(==)>(s: seq<T>, v: T): (o: Option<nat>)
-    ensures if o.Some? then o.value < |s| && s[o.value] == v &&
-                            forall j {:trigger s[j]} :: o.value < j < |s| ==> s[j] != v
-            else v !in s
+  function method {:opaque} LastIndexOfOption<T(==)>(xs: seq<T>, v: T): (o: Option<nat>)
+    ensures if o.Some? then o.value < |xs| && xs[o.value] == v &&
+                            forall j {:trigger xs[j]} :: o.value < j < |xs| ==> xs[j] != v
+            else v !in xs
   {
-    if |s| == 0 then None()
-    else if s[|s|-1] == v then Some(|s| - 1) else LastIndexOfOption(s[..|s|-1], v)
+    if |xs| == 0 then None()
+    else if xs[|xs|-1] == v then Some(|xs| - 1) else LastIndexOfOption(xs[..|xs|-1], v)
   }
 
   /* slices out a specific position's value from the sequence */
-  function method {:opaque} Remove<T>(s: seq<T>, pos: nat): (s': seq<T>)
-    requires pos < |s|
-    ensures |s'| == |s| - 1
-    ensures forall i {:trigger s'[i], s[i]} | 0 <= i < pos :: s'[i] == s[i]
-    ensures forall i {:trigger s'[i]} | pos <= i < |s| - 1 :: s'[i] == s[i+1]
+  function method {:opaque} Remove<T>(xs: seq<T>, pos: nat): (ys: seq<T>)
+    requires pos < |xs|
+    ensures |ys| == |xs| - 1
+    ensures forall i {:trigger ys[i], xs[i]} | 0 <= i < pos :: ys[i] == xs[i]
+    ensures forall i {:trigger ys[i]} | pos <= i < |xs| - 1 :: ys[i] == xs[i+1]
   {
-    s[..pos] + s[pos+1..]
+    xs[..pos] + xs[pos+1..]
   }
 
   /* slices out a specific value from the sequence */
-  function method {:opaque} RemoveValue<T(==)>(s: seq<T>, v: T): (s': seq<T>)
-    ensures v !in s ==> s == s'
-    ensures v in s ==> |multiset(s')| == |multiset(s)| - 1
-    ensures v in s ==> multiset(s')[v] == multiset(s)[v] - 1
-    ensures HasNoDuplicates(s) ==> HasNoDuplicates(s') && ToSet(s') == ToSet(s) - {v}
+  function method {:opaque} RemoveValue<T(==)>(xs: seq<T>, v: T): (ys: seq<T>)
+    ensures v !in xs ==> xs == ys
+    ensures v in xs ==> |multiset(ys)| == |multiset(xs)| - 1
+    ensures v in xs ==> multiset(ys)[v] == multiset(xs)[v] - 1
+    ensures HasNoDuplicates(xs) ==> HasNoDuplicates(ys) && ToSet(ys) == ToSet(xs) - {v}
   {
     reveal HasNoDuplicates();
     reveal ToSet();
-    if v !in s then s
+    if v !in xs then xs
     else
-      var i := IndexOf(s, v);
-      assert s == s[..i] + [v] + s[i+1..];
-      s[..i] + s[i+1..]
+      var i := IndexOf(xs, v);
+      assert xs == xs[..i] + [v] + xs[i+1..];
+      xs[..i] + xs[i+1..]
   }
 
   /* inserts a certain value into a specified index of the sequence */
-  function method {:opaque} Insert<T>(s: seq<T>, a: T, pos: nat): seq<T>
-    requires pos <= |s|
-    ensures |Insert(s, a, pos)| == |s| + 1
-    ensures forall i {:trigger Insert(s, a, pos)[i], s[i]} :: 0 <= i < pos ==> Insert(s, a, pos)[i] == s[i]
-    ensures forall i {:trigger s[i]} :: pos <= i < |s| ==> Insert(s, a, pos)[i+1] == s[i]
-    ensures Insert(s, a, pos)[pos] == a
-    ensures multiset(Insert(s, a, pos)) == multiset(s) + multiset{a}
+  function method {:opaque} Insert<T>(xs: seq<T>, a: T, pos: nat): seq<T>
+    requires pos <= |xs|
+    ensures |Insert(xs, a, pos)| == |xs| + 1
+    ensures forall i {:trigger Insert(xs, a, pos)[i], xs[i]} :: 0 <= i < pos ==> Insert(xs, a, pos)[i] == xs[i]
+    ensures forall i {:trigger xs[i]} :: pos <= i < |xs| ==> Insert(xs, a, pos)[i+1] == xs[i]
+    ensures Insert(xs, a, pos)[pos] == a
+    ensures multiset(Insert(xs, a, pos)) == multiset(xs) + multiset{a}
   {
-    assert s == s[..pos] + s[pos..];
-    s[..pos] + [a] + s[pos..]
+    assert xs == xs[..pos] + xs[pos..];
+    xs[..pos] + [a] + xs[pos..]
   }
 
-  function method {:opaque} Reverse<T>(s: seq<T>): (s': seq<T>)
-    ensures |s'| == |s|
-    ensures forall i {:trigger s'[i]}{:trigger s[|s| - i - 1]} :: 0 <= i < |s| ==> s'[i] == s[|s| - i - 1]
+  function method {:opaque} Reverse<T>(xs: seq<T>): (ys: seq<T>)
+    ensures |ys| == |xs|
+    ensures forall i {:trigger ys[i]}{:trigger xs[|xs| - i - 1]} :: 0 <= i < |xs| ==> ys[i] == xs[|xs| - i - 1]
   {
-    if s == [] then [] else [s[|s|-1]] + Reverse(s[0 .. |s|-1])
+    if xs == [] then [] else [xs[|xs|-1]] + Reverse(xs[0 .. |xs|-1])
   }
     
-  function method {:opaque} Repeat<T>(v: T, length: nat): (s: seq<T>)
-    ensures |s| == length
-    ensures forall i: nat {:trigger s[i]} | i < |s| :: s[i] == v
+  function method {:opaque} Repeat<T>(v: T, length: nat): (xs: seq<T>)
+    ensures |xs| == length
+    ensures forall i: nat {:trigger xs[i]} | i < |xs| :: xs[i] == v
   {
     if length == 0 then
       []
@@ -341,33 +341,33 @@ module Seq {
   }
   
   /* unzips a sequence that contains ordered pairs into 2 seperate sequences */
-  function method {:opaque} Unzip<A,B>(s: seq<(A, B)>): (seq<A>, seq<B>)
-    ensures |Unzip(s).0| == |Unzip(s).1| == |s|
-    ensures forall i {:trigger Unzip(s).0[i]} {:trigger Unzip(s).1[i]} 
-        :: 0 <= i < |s| ==> (Unzip(s).0[i], Unzip(s).1[i]) == s[i]
+  function method {:opaque} Unzip<A,B>(xs: seq<(A, B)>): (seq<A>, seq<B>)
+    ensures |Unzip(xs).0| == |Unzip(xs).1| == |xs|
+    ensures forall i {:trigger Unzip(xs).0[i]} {:trigger Unzip(xs).1[i]} 
+        :: 0 <= i < |xs| ==> (Unzip(xs).0[i], Unzip(xs).1[i]) == xs[i]
   {
-    if |s| == 0 then ([], [])
+    if |xs| == 0 then ([], [])
     else
-      var (a, b):= Unzip(DropLast(s));
-      (a + [Last(s).0], b + [Last(s).1])
+      var (a, b):= Unzip(DropLast(xs));
+      (a + [Last(xs).0], b + [Last(xs).1])
   }
 
-  /* takes two sequences, a and b, and combines then to form one sequence in which
-  each position contains an ordered pair from a and b */
-  function method {:opaque} Zip<A,B>(a: seq<A>, b: seq<B>): seq<(A, B)>
-    requires |a| == |b|
-    ensures |Zip(a, b)| == |a|
-    ensures forall i {:trigger Zip(a, b)[i]}:: 0 <= i < |Zip(a, b)| ==> Zip(a, b)[i] == (a[i], b[i])
-    ensures Unzip(Zip(a, b)).0 == a
-    ensures Unzip(Zip(a, b)).1 == b
+  /* takes two sequences, xs and ys, and combines then to form one sequence in which
+  each position contains an ordered pair from xs and ys */
+  function method {:opaque} Zip<A,B>(xs: seq<A>, ys: seq<B>): seq<(A, B)>
+    requires |xs| == |ys|
+    ensures |Zip(xs, ys)| == |xs|
+    ensures forall i {:trigger Zip(xs, ys)[i]}:: 0 <= i < |Zip(xs, ys)| ==> Zip(xs, ys)[i] == (xs[i], ys[i])
+    ensures Unzip(Zip(xs, ys)).0 == xs
+    ensures Unzip(Zip(xs, ys)).1 == ys
   {
-    if |a| == 0 then []
-    else Zip(DropLast(a), DropLast(b)) + [(Last(a), Last(b))]
+    if |xs| == 0 then []
+    else Zip(DropLast(xs), DropLast(ys)) + [(Last(xs), Last(ys))]
   }
 
   /* if a sequence is unzipped and then zipped, it forms the original sequence */
-  lemma LemmaZipOfUnzip<A,B>(s: seq<(A,B)>)
-    ensures Zip(Unzip(s).0, Unzip(s).1) == s
+  lemma LemmaZipOfUnzip<A,B>(xs: seq<(A,B)>)
+    ensures Zip(Unzip(xs).0, Unzip(xs).1) == xs
   {
   }
 
@@ -378,81 +378,81 @@ module Seq {
   ***********************************************************/
 
   /* finds the maximum integer value in the sequence */
-  function method {:opaque} Max(s: seq<int>): int
-    requires 0 < |s|
-    ensures forall k {:trigger k in s} :: k in s ==> Max(s) >= k
-    ensures Max(s) in s
+  function method {:opaque} Max(xs: seq<int>): int
+    requires 0 < |xs|
+    ensures forall k {:trigger k in xs} :: k in xs ==> Max(xs) >= k
+    ensures Max(xs) in xs
   {
-    assert s == [s[0]] + s[1..];
-    if |s| == 1 then s[0] else Math.Max(s[0], Max(s[1..]))
+    assert xs == [xs[0]] + xs[1..];
+    if |xs| == 1 then xs[0] else Math.Max(xs[0], Max(xs[1..]))
   }
 
-  /* the greater maximum value of two sequences, a and b, becomes the maximum of the total sequence when 
-  a and b are concatenated */
-  lemma LemmaMaxOfConcat(a: seq<int>, b: seq<int>)
-    requires 0 < |a| && 0 < |b|
-    ensures Max(a+b) >= Max(a)
-    ensures Max(a+b) >= Max(b)
-    ensures forall i {:trigger i in [Max(a + b)]} :: i in a + b ==> Max(a + b) >= i
+  /* the greater maximum value of two sequences, xs and ys, becomes the maximum of the total sequence when 
+  xs and ys are concatenated */
+  lemma LemmaMaxOfConcat(xs: seq<int>, ys: seq<int>)
+    requires 0 < |xs| && 0 < |ys|
+    ensures Max(xs+ys) >= Max(xs)
+    ensures Max(xs+ys) >= Max(ys)
+    ensures forall i {:trigger i in [Max(xs + ys)]} :: i in xs + ys ==> Max(xs + ys) >= i
   {
     reveal Max();
-    if |a| == 1 {
+    if |xs| == 1 {
     } else {
-      assert a[1..] + b == (a + b)[1..];
-      LemmaMaxOfConcat(a[1..], b);
+      assert xs[1..] + ys == (xs + ys)[1..];
+      LemmaMaxOfConcat(xs[1..], ys);
     }
   }
 
   /* finds the minimum integer value in the sequence */
-  function method {:opaque} Min(s: seq<int>): int
-    requires 0 < |s|
-    ensures forall k {:trigger k in s} :: k in s ==> Min(s) <= k
-    ensures Min(s) in s
+  function method {:opaque} Min(xs: seq<int>): int
+    requires 0 < |xs|
+    ensures forall k {:trigger k in xs} :: k in xs ==> Min(xs) <= k
+    ensures Min(xs) in xs
   {
-    assert s == [s[0]] + s[1..];
-    if |s| == 1 then s[0] else Math.Min(s[0], Min(s[1..]))
+    assert xs == [xs[0]] + xs[1..];
+    if |xs| == 1 then xs[0] else Math.Min(xs[0], Min(xs[1..]))
   }
 
-  /* the smaller minimum value of two sequences, a and b, becomes the minimum of the total sequence when 
-  a and b are concatenated */
-  lemma LemmaMinOfConcat(a: seq<int>, b: seq<int>)
-    requires 0 < |a| && 0 < |b|
-    ensures Min(a+b) <= Min(a)
-    ensures Min(a+b) <= Min(b)
-    ensures forall i {:trigger i in a + b} :: i in a + b ==> Min(a + b) <= i
+  /* the smaller minimum value of two sequences, xs and ys, becomes the minimum of the total sequence when 
+  xs and ys are concatenated */
+  lemma LemmaMinOfConcat(xs: seq<int>, ys: seq<int>)
+    requires 0 < |xs| && 0 < |ys|
+    ensures Min(xs+ys) <= Min(xs)
+    ensures Min(xs+ys) <= Min(ys)
+    ensures forall i {:trigger i in xs + ys} :: i in xs + ys ==> Min(xs + ys) <= i
   {
     reveal Min();
-    if |a| == 1 {
+    if |xs| == 1 {
     } else {
-      assert a[1..] + b == (a + b)[1..];
-      LemmaMinOfConcat(a[1..], b);
+      assert xs[1..] + ys == (xs + ys)[1..];
+      LemmaMinOfConcat(xs[1..], ys);
     }
   }
 
   /* the maximum element in any subsequence will not be greater than the maximum element in 
   the full sequence */
-  lemma LemmaSubseqMax(s: seq<int>, from: nat, to: nat)
-    requires from < to <= |s|
-    ensures Max(s[from..to]) <= Max(s)
+  lemma LemmaSubseqMax(xs: seq<int>, from: nat, to: nat)
+    requires from < to <= |xs|
+    ensures Max(xs[from..to]) <= Max(xs)
   {
-    var subseq := s[from..to];
-    if Max(subseq) > Max(s) {
+    var subseq := xs[from..to];
+    if Max(subseq) > Max(xs) {
       var k :| 0 <= k < |subseq| && subseq[k] == Max(subseq);
-      assert s[seq(|subseq|, i requires 0 <= i < |subseq| => i + from)[k]] in s;
+      assert xs[seq(|subseq|, i requires 0 <= i < |subseq| => i + from)[k]] in xs;
       assert false;
     }
   }
 
   /* the minimum element in any subsequence will not be less than the minimum element in 
   the full sequence */
-  lemma LemmaSubseqMin(s: seq<int>, from: nat, to: nat)
-    requires from < to <= |s|
-    ensures Min(s[from..to]) >= Min(s)
+  lemma LemmaSubseqMin(xs: seq<int>, from: nat, to: nat)
+    requires from < to <= |xs|
+    ensures Min(xs[from..to]) >= Min(xs)
   {
-    var subseq := s[from..to];
-    if Min(subseq) < Min(s) {
+    var subseq := xs[from..to];
+    if Min(subseq) < Min(xs) {
       var k :| 0 <= k < |subseq| && subseq[k] == Min(subseq);
-      assert s[seq(|subseq|, i requires 0 <= i < |subseq| => i + from)[k]] in s;
+      assert xs[seq(|subseq|, i requires 0 <= i < |subseq| => i + from)[k]] in xs;
     }
   }
 
@@ -464,102 +464,102 @@ module Seq {
 
   /*concatenates a sequence of sequences into a single sequence. Works by adding 
   elements in order from first to last */
-  function method Flatten<T>(s: seq<seq<T>>): seq<T>
-    decreases |s|
+  function method Flatten<T>(xs: seq<seq<T>>): seq<T>
+    decreases |xs|
   {
-    if |s| == 0 then []
-    else s[0] + Flatten(s[1..])
+    if |xs| == 0 then []
+    else xs[0] + Flatten(xs[1..])
   }
 
   /* concatenating two sequences of sequences is equivalent to concatenating 
   each sequence of sequences seperately, and then concatenating the two resulting 
   sequences together */
-  lemma LemmaFlattenConcat<T>(a: seq<seq<T>>, b: seq<seq<T>>)
-    ensures Flatten(a + b) == Flatten(a) + Flatten(b)
+  lemma LemmaFlattenConcat<T>(xs: seq<seq<T>>, ys: seq<seq<T>>)
+    ensures Flatten(xs + ys) == Flatten(xs) + Flatten(ys)
   {
-    if |a| == 0 {
-      assert a + b == b;
+    if |xs| == 0 {
+      assert xs + ys == ys;
     } else {
       calc == {
-        Flatten(a + b);
-          { assert (a + b)[0] == a[0];  assert (a + b)[1..] == a[1..] + b; }
-        a[0] + Flatten(a[1..] + b);
-        a[0] + Flatten(a[1..]) + Flatten(b);
-        Flatten(a) + Flatten(b);
+        Flatten(xs + ys);
+          { assert (xs + ys)[0] == xs[0];  assert (xs + ys)[1..] == xs[1..] + ys; }
+        xs[0] + Flatten(xs[1..] + ys);
+        xs[0] + Flatten(xs[1..]) + Flatten(ys);
+        Flatten(xs) + Flatten(ys);
       }
     }
   }
 
   /* concatenates the sequence of sequences into a single sequence. Works by concatenating 
   elements from last to first */
-  function method FlattenReverse<T>(s: seq<seq<T>>): seq<T>
-  decreases |s|
+  function method FlattenReverse<T>(xs: seq<seq<T>>): seq<T>
+  decreases |xs|
   {
-    if |s| == 0 then []
-    else FlattenReverse(DropLast(s)) + Last(s)
+    if |xs| == 0 then []
+    else FlattenReverse(DropLast(xs)) + Last(xs)
   }
 
   /* concatenating two reversed sequences of sequences is the same as reversing two 
   sequences of sequences and then concattenating the two resulting sequences together */
-  lemma LemmaFlattenReverseConcat<T>(a: seq<seq<T>>, b: seq<seq<T>>)
-  ensures FlattenReverse(a + b) == FlattenReverse(a) + FlattenReverse(b)
+  lemma LemmaFlattenReverseConcat<T>(xs: seq<seq<T>>, ys: seq<seq<T>>)
+  ensures FlattenReverse(xs + ys) == FlattenReverse(xs) + FlattenReverse(ys)
   {
-    if |b| == 0 {
-      assert FlattenReverse(b) == [];
-      assert a + b == a;
+    if |ys| == 0 {
+      assert FlattenReverse(ys) == [];
+      assert xs + ys == xs;
     } else {
       calc == {
-        FlattenReverse(a + b);
-          { assert Last(a + b) == Last(b);  assert DropLast(a + b) == a + DropLast(b); }
-        FlattenReverse(a + DropLast(b)) + Last(b);
-        FlattenReverse(a) + FlattenReverse(DropLast(b)) + Last(b);
-        FlattenReverse(a) + FlattenReverse(b);
+        FlattenReverse(xs + ys);
+          { assert Last(xs + ys) == Last(ys);  assert DropLast(xs + ys) == xs + DropLast(ys); }
+        FlattenReverse(xs + DropLast(ys)) + Last(ys);
+        FlattenReverse(xs) + FlattenReverse(DropLast(ys)) + Last(ys);
+        FlattenReverse(xs) + FlattenReverse(ys);
       }
     }
   }
 
   /* both methods of concatenating sequence (starting from front v. starting from back)
   result in the same sequence */
-  lemma LemmaFlattenAndFlattenReverseAreEquivalent<T>(s: seq<seq<T>>)
-    ensures Flatten(s) == FlattenReverse(s)
+  lemma LemmaFlattenAndFlattenReverseAreEquivalent<T>(xs: seq<seq<T>>)
+    ensures Flatten(xs) == FlattenReverse(xs)
   {
-    if |s| == 0 {
+    if |xs| == 0 {
     } else {
       calc == {
-        FlattenReverse(s);
-        FlattenReverse(DropLast(s)) + Last(s);
-          { LemmaFlattenAndFlattenReverseAreEquivalent(DropLast(s)); }
-        Flatten(DropLast(s)) + Last(s);
-        Flatten(DropLast(s)) + Flatten([Last(s)]);
-          { LemmaFlattenConcat(DropLast(s), [Last(s)]); 
-        assert s == DropLast(s) + [Last(s)]; }
-        Flatten(s);
+        FlattenReverse(xs);
+        FlattenReverse(DropLast(xs)) + Last(xs);
+          { LemmaFlattenAndFlattenReverseAreEquivalent(DropLast(xs)); }
+        Flatten(DropLast(xs)) + Last(xs);
+        Flatten(DropLast(xs)) + Flatten([Last(xs)]);
+          { LemmaFlattenConcat(DropLast(xs), [Last(xs)]); 
+        assert xs == DropLast(xs) + [Last(xs)]; }
+        Flatten(xs);
       }
     }
   }
 
   /* the concatenated sequence's length is greater than or equal to each individual
   inner sequence's length */
-  lemma LemmaFlattenLengthGeSingleElementLength<T>(s: seq<seq<T>>, i: int)
-    requires 0 <= i < |s|
-    ensures |FlattenReverse(s)| >= |s[i]|
+  lemma LemmaFlattenLengthGeSingleElementLength<T>(xs: seq<seq<T>>, i: int)
+    requires 0 <= i < |xs|
+    ensures |FlattenReverse(xs)| >= |xs[i]|
   {
-    if i < |s| - 1 {
-      LemmaFlattenLengthGeSingleElementLength(s[..|s|-1], i);
+    if i < |xs| - 1 {
+      LemmaFlattenLengthGeSingleElementLength(xs[..|xs|-1], i);
     }
   }
 
   /* the length of concatenating sequence in a sequence together will be no longer 
   than the length of the original sequence of sequences multiplied by the length of 
   the longest sequence */
-  lemma LemmaFlattenLengthLeMul<T>(s: seq<seq<T>>, j: int)
-    requires forall i {:trigger s[i]} | 0 <= i < |s| :: |s[i]| <= j
-    ensures |FlattenReverse(s)| <= |s| * j
+  lemma LemmaFlattenLengthLeMul<T>(xs: seq<seq<T>>, j: int)
+    requires forall i {:trigger xs[i]} | 0 <= i < |xs| :: |xs[i]| <= j
+    ensures |FlattenReverse(xs)| <= |xs| * j
   {
-    if |s| == 0 {
+    if |xs| == 0 {
     } else {
-      LemmaFlattenLengthLeMul(s[..|s|-1], j);
-      assert |FlattenReverse(s[..|s|-1])| <= (|s|-1) * j;
+      LemmaFlattenLengthLeMul(xs[..|xs|-1], j);
+      assert |FlattenReverse(xs[..|xs|-1])| <= (|xs|-1) * j;
     }
   }
 
@@ -571,115 +571,115 @@ module Seq {
   ***********************************************************/
 
   /* applies a transformation function on the sequence */
-  function method {:opaque} Map<T,R>(f: (T ~> R), s: seq<T>): (result: seq<R>)
-    requires forall i {:trigger s[i]} :: 0 <= i < |s| ==> f.requires(s[i])
-    ensures |result| == |s|
-    ensures forall i {:trigger result[i]}:: 0 <= i < |s| ==> result[i] == f(s[i]);
-    reads set i, o {:trigger o in f.reads(s[i])} | 0 <= i < |s| && o in f.reads(s[i]):: o
+  function method {:opaque} Map<T,R>(f: (T ~> R), xs: seq<T>): (result: seq<R>)
+    requires forall i {:trigger xs[i]} :: 0 <= i < |xs| ==> f.requires(xs[i])
+    ensures |result| == |xs|
+    ensures forall i {:trigger result[i]}:: 0 <= i < |xs| ==> result[i] == f(xs[i]);
+    reads set i, o {:trigger o in f.reads(xs[i])} | 0 <= i < |xs| && o in f.reads(xs[i]):: o
   {
-    if |s| == 0 then []
-    else [f(s[0])] + Map(f, s[1..])
+    if |xs| == 0 then []
+    else [f(xs[0])] + Map(f, xs[1..])
   }
 
 /* applies a transformation function that returns a result on the sequence */
-  function method {:opaque} MapWithResult<T, R, E>(f: (T ~> Result<R,E>), s: seq<T>): (result: Result<seq<R>, E>)
-    requires forall i :: 0 <= i < |s| ==> f.requires(s[i])
+  function method {:opaque} MapWithResult<T, R, E>(f: (T ~> Result<R,E>), xs: seq<T>): (result: Result<seq<R>, E>)
+    requires forall i :: 0 <= i < |xs| ==> f.requires(xs[i])
     ensures result.Success? ==>
-      && |result.value| == |s|
-      && (forall i :: 0 <= i < |s| ==> 
-        && f(s[i]).Success?
-        && result.value[i] == f(s[i]).value)
-    reads set i, o | 0 <= i < |s| && o in f.reads(s[i]) :: o
+      && |result.value| == |xs|
+      && (forall i :: 0 <= i < |xs| ==> 
+        && f(xs[i]).Success?
+        && result.value[i] == f(xs[i]).value)
+    reads set i, o | 0 <= i < |xs| && o in f.reads(xs[i]) :: o
   {
-    if |s| == 0 then Success([])
+    if |xs| == 0 then Success([])
     else
-      var head :- f(s[0]);
-      var tail :- MapWithResult(f, s[1..]);
+      var head :- f(xs[0]);
+      var tail :- MapWithResult(f, xs[1..]);
       Success([head] + tail)
   }
 
   /* concatenating two sequences and then applying Map is the same as applying
   Map on each sequence  seperately and then concatenating the two resulting
   sequences */
-  lemma {:opaque} LemmaMapDistributesOverConcat<T,R>(f: (T ~> R), a: seq<T>, b: seq<T>)
-    requires forall i {:trigger a[i]}:: 0 <= i < |a| ==> f.requires(a[i])
-    requires forall j {:trigger b[j]}:: 0 <= j < |b| ==> f.requires(b[j])
-    ensures Map(f, a + b) == Map(f, a) + Map(f, b)
+  lemma {:opaque} LemmaMapDistributesOverConcat<T,R>(f: (T ~> R), xs: seq<T>, ys: seq<T>)
+    requires forall i {:trigger xs[i]}:: 0 <= i < |xs| ==> f.requires(xs[i])
+    requires forall j {:trigger ys[j]}:: 0 <= j < |ys| ==> f.requires(ys[j])
+    ensures Map(f, xs + ys) == Map(f, xs) + Map(f, ys)
   {
     reveal Map();
-    if |a| == 0 {
-      assert a + b == b;
+    if |xs| == 0 {
+      assert xs + ys == ys;
     } else {
       calc {
-        Map(f, a + b);
-          { assert (a + b)[0] == a[0]; assert (a + b)[1..] == a[1..] + b; }
-        Map(f, [a[0]]) + Map(f, a[1..] + b);
-        Map(f, [a[0]]) + Map(f, a[1..]) + Map(f, b);
-          {assert [(a + b)[0]] + a[1..] + b == a + b;}
-        Map(f, a) + Map(f, b);
+        Map(f, xs + ys);
+          { assert (xs + ys)[0] == xs[0]; assert (xs + ys)[1..] == xs[1..] + ys; }
+        Map(f, [xs[0]]) + Map(f, xs[1..] + ys);
+        Map(f, [xs[0]]) + Map(f, xs[1..]) + Map(f, ys);
+          {assert [(xs + ys)[0]] + xs[1..] + ys == xs + ys;}
+        Map(f, xs) + Map(f, ys);
       }
     }
   }
 
   /* uses a selection function to select elements from the sequence */
-  function method {:opaque} Filter<T>(f: (T ~> bool), s: seq<T>): (result: seq<T>)
-    requires forall i :: 0 <= i < |s| ==> f.requires(s[i])
-    ensures |result| <= |s|
+  function method {:opaque} Filter<T>(f: (T ~> bool), xs: seq<T>): (result: seq<T>)
+    requires forall i :: 0 <= i < |xs| ==> f.requires(xs[i])
+    ensures |result| <= |xs|
     ensures forall i: nat {:trigger result[i]} :: i < |result| && f.requires(result[i]) ==> f(result[i])
     reads f.reads
   {
-    if |s| == 0 then []
-    else (if f(s[0]) then [s[0]] else []) + Filter(f, s[1..])
+    if |xs| == 0 then []
+    else (if f(xs[0]) then [xs[0]] else []) + Filter(f, xs[1..])
   }
 
   /* concatenating two sequences and then using "filter" is the same as using "filter" on each sequences
   seperately and then concatenating their resulting sequences */
-  lemma {:opaque} LemmaFilterDistributesOverConcat<T>(f: (T ~> bool), a: seq<T>, b: seq<T>)
-    requires forall i {:trigger a[i]}:: 0 <= i < |a| ==> f.requires(a[i])
-    requires forall j {:trigger b[j]}:: 0 <= j < |b| ==> f.requires(b[j])
-    ensures Filter(f, a + b) == Filter(f, a) + Filter(f, b)
+  lemma {:opaque} LemmaFilterDistributesOverConcat<T>(f: (T ~> bool), xs: seq<T>, ys: seq<T>)
+    requires forall i {:trigger xs[i]}:: 0 <= i < |xs| ==> f.requires(xs[i])
+    requires forall j {:trigger ys[j]}:: 0 <= j < |ys| ==> f.requires(ys[j])
+    ensures Filter(f, xs + ys) == Filter(f, xs) + Filter(f, ys)
   {
     reveal Filter();
-    if |a| == 0 {
-      assert a + b == b;
+    if |xs| == 0 {
+      assert xs + ys == ys;
     } else {
       calc {
-        Filter(f, a + b);
-          { assert (a + b)[0] == a[0]; assert (a + b)[1..] == a[1..] + b; }
-        Filter(f, [a[0]]) + Filter(f, a[1..] + b);
-        Filter(f, [a[0]]) + Filter(f, a[1..]) + Filter(f, b);
-          { assert [(a + b)[0]] + a[1..] + b == a + b; }
-        Filter(f, a) + Filter(f, b);
+        Filter(f, xs + ys);
+          { assert (xs + ys)[0] == xs[0]; assert (xs + ys)[1..] == xs[1..] + ys; }
+        Filter(f, [xs[0]]) + Filter(f, xs[1..] + ys);
+        Filter(f, [xs[0]]) + Filter(f, xs[1..]) + Filter(f, ys);
+          { assert [(xs + ys)[0]] + xs[1..] + ys == xs + ys; }
+        Filter(f, xs) + Filter(f, ys);
       }
     }
   }
   
-  function method {:opaque} FoldLeft<A,T>(f: (A, T) -> A, init: A, s: seq<T>): A
+  function method {:opaque} FoldLeft<A,T>(f: (A, T) -> A, init: A, xs: seq<T>): A
   {
-    if |s| == 0 then init
-    else FoldLeft(f, f(init, s[0]), s[1..])
+    if |xs| == 0 then init
+    else FoldLeft(f, f(init, xs[0]), xs[1..])
   }
 
   /* Concatenating two sequences, then folding left is the same as folding the first sequence and using the result as the initial value to fold the second
   sequence. */
-  lemma {:opaque} LemmaFoldLeftDistributesOverConcat<A,T>(f: (A, T) -> A, init: A, a: seq<T>, b: seq<T>)
-    requires 0 <= |a + b|
-    ensures FoldLeft(f, init, a + b) == FoldLeft(f, FoldLeft(f, init, a), b)
+  lemma {:opaque} LemmaFoldLeftDistributesOverConcat<A,T>(f: (A, T) -> A, init: A, xs: seq<T>, ys: seq<T>)
+    requires 0 <= |xs + ys|
+    ensures FoldLeft(f, init, xs + ys) == FoldLeft(f, FoldLeft(f, init, xs), ys)
   {
     reveal FoldLeft();
-    if |a| == 0 {
-      assert a + b == b;
+    if |xs| == 0 {
+      assert xs + ys == ys;
     } else {
-      assert |a| >= 1;
-      assert ([a[0]] + a[1..] + b)[0] == a[0];
+      assert |xs| >= 1;
+      assert ([xs[0]] + xs[1..] + ys)[0] == xs[0];
       calc {
-        FoldLeft(f, FoldLeft(f, init, a), b);
-        FoldLeft(f, FoldLeft(f, f(init, a[0]), a[1..]), b);
-          { LemmaFoldLeftDistributesOverConcat(f, f(init, a[0]), a[1..], b); }
-        FoldLeft(f, f(init, a[0]), a[1..] + b);
-          { assert (a + b)[0] == a[0];
-            assert (a + b)[1..] == a[1..] + b; }
-        FoldLeft(f, init, a + b);
+        FoldLeft(f, FoldLeft(f, init, xs), ys);
+        FoldLeft(f, FoldLeft(f, f(init, xs[0]), xs[1..]), ys);
+          { LemmaFoldLeftDistributesOverConcat(f, f(init, xs[0]), xs[1..], ys); }
+        FoldLeft(f, f(init, xs[0]), xs[1..] + ys);
+          { assert (xs + ys)[0] == xs[0];
+            assert (xs + ys)[1..] == xs[1..] + ys; }
+        FoldLeft(f, init, xs + ys);
       }
     }
   }
@@ -712,29 +712,29 @@ module Seq {
     }
   }
 
-  function method {:opaque} FoldRight<A,T>(f: (T, A) -> A, s: seq<T>, init: A): A
+  function method {:opaque} FoldRight<A,T>(f: (T, A) -> A, xs: seq<T>, init: A): A
   {
-    if |s| == 0 then init
-    else f(s[0], FoldRight(f, s[1..], init))
+    if |xs| == 0 then init
+    else f(xs[0], FoldRight(f, xs[1..], init))
   }
 
   /* Concatenating two sequences, then folding right is the same as folding the second sequence and using the result as the initial value to fold the first
   sequence. */
-  lemma {:opaque} LemmaFoldRightDistributesOverConcat<A,T>(f: (T, A) -> A, init: A, a: seq<T>, b: seq<T>)
-    requires 0 <= |a + b|
-    ensures FoldRight(f, a + b, init) == FoldRight(f, a, FoldRight(f, b, init))
+  lemma {:opaque} LemmaFoldRightDistributesOverConcat<A,T>(f: (T, A) -> A, init: A, xs: seq<T>, ys: seq<T>)
+    requires 0 <= |xs + ys|
+    ensures FoldRight(f, xs + ys, init) == FoldRight(f, xs, FoldRight(f, ys, init))
   {
     reveal FoldRight();
-    if |a| == 0 {
-      assert a + b == b;
+    if |xs| == 0 {
+      assert xs + ys == ys;
     } else {
       calc {
-        FoldRight(f, a, FoldRight(f, b, init));
-        f(a[0], FoldRight(f, a[1..], FoldRight(f, b, init)));
-        f(a[0], FoldRight(f, a[1..] + b, init));
-          { assert (a + b)[0] == a[0];
-            assert (a + b)[1..] == a[1..] + b; }
-        FoldRight(f, a + b, init);
+        FoldRight(f, xs, FoldRight(f, ys, init));
+        f(xs[0], FoldRight(f, xs[1..], FoldRight(f, ys, init)));
+        f(xs[0], FoldRight(f, xs[1..] + ys, init));
+          { assert (xs + ys)[0] == xs[0];
+            assert (xs +ys)[1..] == xs[1..] + ys; }
+        FoldRight(f, xs + ys, init);
       }
     }
   }
